Pyramid.fst
@@ -30,6 +30,18 @@ let address_to_uint a =
 val uint_to_address : UInt256.t -> UInt160.t
 let uint_to_address a = UInt160.uint_to_t (UInt.to_uint_t 160 (UInt256.v a))
 
+val default_address : UInt160.t
+let default_address = UInt160.uint_to_t 0
+
+val default_uint256 : UInt256.t
+let default_uint256 = UInt256.uint_to_t 0
+
+val default_uint : UInt256.t
+let default_uint = UInt256.uint_to_t 0
+
+val default_bool : bool
+let default_bool = false
+
 val list_length : #a:Type -> list a -> UInt256.t
 let list_length #a lst = UInt256.uint_to_t (UInt.to_uint_t 256 (List.length lst))
 
@@ -73,6 +85,14 @@ balance : UInt160.t -> UInt256.t;
 invite : UInt160.t -> UInt160.t;
 invites_left : UInt160.t -> UInt256.t;
 joined : UInt160.t -> bool;
+}
+let default_state = {
+events__ = []; balance__ = (fun x -> default_uint);
+parent = (fun x -> default_address);
+balance = (fun x -> default_uint);
+invite = (fun x -> default_address);
+invites_left = (fun x -> default_uint);
+joined = (fun x -> default_bool);
 }
 let uint256_10 = UInt256.uint_to_t (10)
 let address_0 = UInt160.uint_to_t (0)
