Token.fst
@@ -30,6 +30,15 @@ let address_to_uint a =
 val uint_to_address : UInt256.t -> UInt160.t
 let uint_to_address a = UInt160.uint_to_t (UInt.to_uint_t 160 (UInt256.v a))
 
+val default_address : UInt160.t
+let default_address = UInt160.uint_to_t 0
+
+val default_uint256 : UInt256.t
+let default_uint256 = UInt256.uint_to_t 0
+
+val default_uint : UInt256.t
+let default_uint = UInt256.uint_to_t 0
+
 val list_length : #a:Type -> list a -> UInt256.t
 let list_length #a lst = UInt256.uint_to_t (UInt.to_uint_t 256 (List.length lst))
 
@@ -69,6 +78,10 @@ type event = unit
 noeq type state = {
 events__: list event; balance__ : UInt160.t -> UInt256.t;
 balance : UInt160.t -> UInt256.t;
+}
+let default_state = {
+events__ = []; balance__ = (fun x -> default_uint);
+balance = (fun x -> default_uint);
 }
 assume type inv : state -> Type
 assume val call_env : state -> state
